# Newton's Law of Universal Gravitation
By messing around with an apple and the moon, newton discovered:
> $a$ ∝ $\frac{1}{R^2}$ (R = distance from centre of earth.)
> This is the inverse square law.

Therefore:
> $F$ ∝ $\frac{m}{R^2}$
> Finally:
> $F$ ∝ $\frac{Mm}{R^2}$ (M, m = masses of two objects) (R = distance between them)

We can get rid of the proportionality symbol by introducing a constant.

### Final Formula
> $F = \frac{GMm}{R^2}$ (F is the force exerted on an object by gravity)
> G is the gravitational constant.
> G = $6.67$x$10^{-11}Nm^2kg^{-2}$

Since gravity is an attractive force, we can say that the gravitational field strength g is $-\frac{GMm}{R^2}$